lift: Prove lift_scheduler and lift_action lemmas

examples/dynamic_isolation/Interp.v
@@ -5,6 +5,8 @@ Require Import Koika.Syntax.
 Require Import Koika.TypedSemantics.
 Require Import Koika.TypedSyntax.
 
+Require Import dynamic_isolation.Tactics.
+
 Section Interp.
   Context {pos_t var_t fn_name_t rule_name_t reg_t ext_fn_t: Type}.
   Context {reg_t_eq_dec: EqDec reg_t}.
@@ -23,6 +25,14 @@ Section Interp.
   Notation scheduler := (scheduler pos_t rule_name_t).
   Notation interp_rule := (interp_rule r sigma).
 
+  Fixpoint schedule_app (sched1: scheduler) (sched2: scheduler) : scheduler :=
+    match sched1 with
+    | Done => sched2
+    | Cons r s => Cons r (schedule_app s sched2)
+    | Try r s1 s2 => Try r (schedule_app s1 sched2) (schedule_app s2 sched2)
+    | SPos v s => SPos (rule_name_t := rule_name_t) v (schedule_app s sched2)
+    end.
+
   Section Scheduler.
     Context (rules: rule_name_t -> rule).
 
@@ -32,8 +42,8 @@ Section Interp.
              (s: scheduler)
              {struct s} :=
       let interp_try r s1 s2 :=
-          match interp_rule sched_log (rules r) with
-          | Some l => interp_scheduler_delta' (log_app l sched_log) (log_app l acc_log) s1
+          match interp_rule (log_app acc_log sched_log) (rules r) with
+          | Some l => interp_scheduler_delta' sched_log (log_app l acc_log) s1
           | None => interp_scheduler_delta' sched_log acc_log s2
           end in
       match s with
@@ -47,4 +57,79 @@ Section Interp.
       interp_scheduler_delta' sched_log log_empty s.
 
   End Scheduler.
+
+  Section Lemmas.
+    Context (rules: rule_name_t -> rule).
+
+    Notation interp_scheduler' := (interp_scheduler' r sigma rules).
+    Notation interp_scheduler_delta' := (interp_scheduler_delta' rules).
+    Notation interp_scheduler_delta := (interp_scheduler_delta rules).
+
+    Lemma interp_scheduler'_app :
+      forall (sched1 sched2: scheduler) (log: Log),
+      interp_scheduler' log (schedule_app sched1 sched2) =
+        interp_scheduler' (interp_scheduler' log sched1) sched2.
+    Proof.
+      induction sched1; auto.
+      - intros; simpl.
+        repeat rewrite IHsched1.
+        destruct_goal_matches.
+      - intros; simpl.
+        repeat rewrite IHsched1_1.
+        repeat rewrite IHsched1_2.
+        destruct_goal_matches; auto.
+    Qed.
+
+    Hint Rewrite @SemanticProperties.log_app_assoc : log_rewrites.
+    Hint Rewrite @SemanticProperties.log_app_empty_r : log_rewrites.
+
+
+    Lemma interp_scheduler'_delta_log_app :
+      forall sched l1 l2 l3,
+      interp_scheduler_delta' l2 (log_app l3 l1) sched =
+      log_app (interp_scheduler_delta' (log_app l1 l2) l3 sched) l1.
+    Proof.
+      induction sched; auto.
+      - intros; simpl.
+        autorewrite with log_rewrites; destruct_goal_matches.
+        autorewrite with log_rewrites; auto.
+      - intros; simpl.
+        autorewrite with log_rewrites; destruct_goal_matches.
+        autorewrite with log_rewrites; auto.
+    Qed.
+
+    Lemma interp_scheduler_delta'_correspond_to_interp_scheduler' :
+      forall (sched: scheduler) (sched_log: Log) (acc_log: Log),
+      interp_scheduler' (log_app acc_log sched_log) sched =
+        log_app (interp_scheduler_delta' sched_log acc_log sched) sched_log.
+    Proof.
+      induction sched; auto.
+      - intros; simpl.
+        destruct_goal_matches.
+        repeat rewrite IHsched.
+        rewrite interp_scheduler'_delta_log_app.
+        autorewrite with log_rewrites; auto.
+      - intros; simpl.
+        destruct_goal_matches.
+        repeat rewrite IHsched1.
+        rewrite interp_scheduler'_delta_log_app.
+        autorewrite with log_rewrites; auto.
+     Qed.
+
+    Lemma interp_scheduler_delta_correspond_to_interp_scheduler :
+      forall (sched: scheduler) (sched_log: Log) ,
+      interp_scheduler' sched_log sched =
+        log_app (interp_scheduler_delta sched_log sched) sched_log.
+    Proof.
+      intros. unfold interp_scheduler_delta.
+      rewrite<-interp_scheduler_delta'_correspond_to_interp_scheduler'.
+      autorewrite with log_rewrites. auto.
+    Qed.
+
+  End Lemmas.
+
 End Interp.
+
+Notation "r '||>' s" :=
+  (schedule_app r s)
+    (at level 99, s at level 99, right associativity).
