examples/dynamic_isolation/Lift.v
@@ -1,4 +1,5 @@
 Require Import Koika.Frontend.
+Require Import dynamic_isolation.Interp.
 Require Import dynamic_isolation.Tactics.
 Require Import Coq.Program.Equality.
 
@@ -48,6 +49,9 @@ Section Inverse.
 
 End Inverse.
 
+Hint Rewrite @getenv_create : log_helpers.
+Hint Rewrite @getenv_map2 : log_helpers.
+
 Section ScheduleLift.
   Context {pos_t : Type} {rule_name_t : Type} {rule_name_t' : Type}.
   Context (lift: rule_name_t -> rule_name_t').
@@ -61,19 +65,7 @@ Section ScheduleLift.
     | SPos pos s => SPos pos (lift_scheduler s)
     end.
 
-  Fixpoint schedule_app {rule_name_t: Type} (sched1: scheduler) (sched2: scheduler) : scheduler :=
-    match sched1 with
-    | Done => sched2
-    | Cons r s => Cons r (schedule_app s sched2)
-    | Try r s1 s2 => Try r (schedule_app s1 sched2) (schedule_app s2 sched2)
-    | SPos v s => SPos (rule_name_t := rule_name_t) v (schedule_app s sched2)
-    end.
-
 End ScheduleLift.
-
-Notation "r '||>' s" :=
-  (schedule_app r s)
-    (at level 99, s at level 99, right associativity).
 
 Section Lift.
   Context {reg_t reg_t' : Type}.
@@ -81,8 +73,10 @@ Section Lift.
   Context {REnv: Env reg_t} {REnv': Env reg_t'}.
   Context (Rlift: RLift type reg_t reg_t' R R').
 
-  Context {FT_R : FiniteType reg_t}.
-  Context {EqDec_R' : EqDec reg_t'}.
+  Context {FT_reg_t : FiniteType reg_t}.
+  Context {EqDec_reg_t : EqDec reg_t}.
+  Context {EqDec_reg_t' : EqDec reg_t'}.
+
 
   Section LiftEnv.
     Definition proj_env (env': env_t REnv' R') : env_t REnv R.
@@ -112,8 +106,6 @@ Section Lift.
                                        getenv REnv' log' (Rlift.(rlift) reg)).
   End LiftLog.
 
-  Hint Rewrite @getenv_create : log_helpers.
-
   Section Lemmas.
     Lemma getenv_proj_log :
       forall log' r,
@@ -126,6 +118,38 @@ Section Lift.
       autorewrite with log_helpers.
       auto.
     Qed.
+
+    Lemma getenv_proj_env :
+      forall st' r,
+      getenv REnv (proj_env st') r =
+        (rew <- [fun t : type => t -> R r] pf_R_equal Rlift r in (fun x : R r => x))
+          (getenv REnv' st' (rlift Rlift r)).
+    Proof.
+      intros. unfold proj_env.
+      autorewrite with log_helpers.
+      elim_eq_rect.
+      auto.
+    Qed.
+
+    Lemma putenv_proj_log :
+      forall log' r rlog,
+      putenv REnv (proj_log log') r rlog =
+        proj_log
+            (putenv REnv' log' (Rlift.(rlift) r) (rew <- [fun t : type => RLog t] pf_R_equal Rlift r in rlog)).
+    Proof.
+      intros. apply equiv_eq; unfold equiv. intro k.
+      destruct EqDec_reg_t.
+      destruct (eq_dec r k); subst.
+      - rewrite get_put_eq. rewrite getenv_proj_log. rewrite get_put_eq.
+        destruct (pf_R_equal Rlift k); simpl; auto.
+      - rewrite get_put_neq; auto. rewrite getenv_proj_log.
+        rewrite getenv_proj_log. destruct (pf_R_equal Rlift k).
+        simpl; auto. rewrite get_put_neq; auto.
+        destruct EqDec_reg_t'.
+        destruct (eq_dec0 (rlift Rlift r) (rlift Rlift k)); auto.
+        apply (pf_inj_rlift Rlift) in e. contradiction.
+    Qed.
+
 
     Lemma latest_write_proj_log :
       (forall log' r,
@@ -157,13 +181,60 @@ Section Lift.
       elim_eq_rect; simpl; auto.
     Qed.
 
+    Lemma proj_log_empty :
+      proj_log log_empty = log_empty.
+    Proof.
+      apply equiv_eq.
+      unfold equiv, proj_log.
+      intros.
+      unfold log_empty.
+      autorewrite with log_helpers.
+      elim_eq_rect; simpl; auto.
+    Qed.
+
+    Lemma log_app_comm_proj_log :
+      forall (log1 log2: Log R' REnv'),
+      log_app (R := R) (REnv := REnv) (proj_log log1) (proj_log log2) =
+      proj_log (log_app (R := R') log1 log2).
+    Proof.
+      intros. apply equiv_eq.
+      unfold log_app, proj_log, equiv.
+      intros.
+      autorewrite with log_helpers.
+      elim_eq_rect; auto.
+    Qed.
+
+    Lemma may_read_proj_eq_may_read_lift :
+      forall (log': Log R' REnv') port idx,
+      may_read (proj_log log') port idx = may_read (REnv := REnv') log' port (rlift Rlift idx).
+    Proof.
+      intros; unfold may_read, log_existsb.
+      destruct port; repeat rewrite getenv_proj_log; elim_eq_rect; auto.
+    Qed.
+
+    Lemma may_write_proj_eq_may_write_lift :
+      forall (log1 log2: Log R' REnv') port idx,
+      may_write (proj_log log1) (proj_log log2) port idx = may_write (REnv := REnv') log1 log2 port (rlift Rlift idx).
+    Proof.
+      intros; unfold may_write, log_existsb.
+      destruct port; rewrite log_app_comm_proj_log; rewrite getenv_proj_log;
+        elim_eq_rect; auto.
+    Qed.
+
   End Lemmas.
 
 End Lift.
 
+Hint Rewrite @Lift.getenv_proj_log : log_helpers.
+Hint Rewrite @Lift.putenv_proj_log : log_helpers.
+Hint Rewrite @Lift.getenv_proj_env : log_helpers.
+Hint Rewrite @Lift.getenv_proj_log : log_helpers.
 Hint Rewrite @Lift.latest_write_proj_log : log_helpers.
 Hint Rewrite @Lift.latest_write0_proj_log : log_helpers.
 Hint Rewrite @Lift.latest_write1_proj_log : log_helpers.
+Hint Rewrite @Lift.proj_log_empty : log_helpers.
+Hint Rewrite @Lift.log_app_comm_proj_log : log_helpers. (* TODO: make hint work *)
+Hint Rewrite @Lift.may_read_proj_eq_may_read_lift : log_helpers. (* TODO: make hint work *)
 
 Section LiftAction.
   Context {reg_t reg_t' : Type}.
@@ -176,7 +247,7 @@ Section LiftAction.
   Context {Sigma': ext_fn_t' -> ExternalSignature}.
   Context (Fnlift : RLift ExternalSignature ext_fn_t ext_fn_t' Sigma Sigma').
 
-  Definition lift := Rlift.(rlift).
+  Notation lift := Rlift.(rlift).
 
   Section Args.
     Context (lift_action:
@@ -236,6 +307,292 @@ Section LiftAction.
       lift_action rl.
 
 End LiftAction.
+
+Section Properties_LiftSchedule.
+  Context {rule_name_t rule_name_t' reg_t reg_t' ext_fn_t ext_fn_t': Type}.
+  Context {R: reg_t -> type} {R' : reg_t' -> type}.
+  Context (Rlift: RLift type reg_t reg_t' R R').
+
+  Context {Sigma: ext_fn_t -> ExternalSignature} {Sigma': ext_fn_t' -> ExternalSignature}.
+  Context (Fnlift : RLift ExternalSignature ext_fn_t ext_fn_t' Sigma Sigma').
+  Context (sigma: forall f, Sig_denote (Sigma f)) (sigma': forall f, Sig_denote (Sigma' f)).
+
+  Context {REnv: Env reg_t} {REnv': Env reg_t'}.
+  Context (r: REnv.(env_t) R) (r': REnv'.(env_t) R').
+
+  Context (rule_name_lift: rule_name_t -> rule_name_t').
+
+  Context {FT_reg_t : FiniteType reg_t}.
+  Context {EqDec_reg_t : EqDec reg_t}.
+  Context {EqDec_reg_t' : EqDec reg_t'}.
+
+  Notation rule' := (rule R' Sigma').
+  Notation rule := (rule R Sigma).
+  Notation action' := (action R' Sigma').
+  Notation action := (action R Sigma).
+  Notation schedule' := (scheduler rule_name_t').
+  Notation schedule := (scheduler rule_name_t).
+
+  Notation interp_rule := (interp_rule (fn_name_t := fn_name_t)).
+  Notation lift_action := (lift_action Rlift Fnlift).
+  Notation lift_rule := (lift_rule Rlift Fnlift).
+  Notation proj_log := (proj_log (REnv := REnv) Rlift).
+  Notation proj_env := (proj_env (REnv := REnv) Rlift).
+  Context (rules: rule_name_t -> rule) (rules': rule_name_t' -> rule').
+
+  Definition proj_interp_action_result {sig: tsig var_t} {ret_ty: type}
+                                (res': option (Log R' REnv' * ret_ty * (tcontext sig)))
+                                : option (Log R REnv * ret_ty * (tcontext sig)) :=
+    match res' with
+    | None => None
+    | Some (v1, v2, v3) => Some (proj_log v1, v2, v3)
+    end.
+
+  Section LiftActionPreserves.
+
+    Ltac _start := simpl; unfold opt_bind, proj_interp_action_result in *; intros; auto.
+    Ltac _destruct := match_innermost_in_goal; destruct_pairs; auto.
+
+    Fixpoint lift_action_preserves {sig: tsig var_t}
+                                   {ret_ty : type}
+                                   (action: action sig ret_ty)
+                                   {struct action}:
+      forall
+        (st': REnv'.(env_t) (fun idx: reg_t' => R' idx))
+        (sched_log: Log R' REnv') (action_log: Log R' REnv') (gamma: tcontext sig),
+      (forall f, Sigma f = Sigma' (Fnlift.(rlift) f)) ->
+      (forall f, sigma f = rew [fun e : ExternalSignature => Sig_denote e] pf_R_equal Fnlift f in sigma' (Fnlift.(rlift) f)) ->
+      interp_action (proj_env st') sigma gamma (proj_log sched_log) (proj_log action_log) action =
+      proj_interp_action_result (interp_action st' sigma' gamma sched_log action_log (lift_action action)).
+
+    Proof.
+      * destruct action.
+        (* Fail *)
+        - _start.
+        (* Var *)
+        - _start.
+        (* Const *)
+        - _start.
+        (* Assign *)
+        - _start.
+          rewrite lift_action_preserves; auto.
+          _destruct.
+        (* Seq *)
+        - _start.
+          rewrite lift_action_preserves; auto.
+          _destruct.
+        (* Bind *)
+        - _start.
+          rewrite lift_action_preserves; auto.
+          _destruct.
+          rewrite lift_action_preserves; auto.
+          _destruct.
+        (* If *)
+        - _start.
+          rewrite lift_action_preserves; auto.
+          _destruct.
+          _destruct.
+        (* Read *)
+        - _start.
+          destruct port; simpl.
+          + _destruct.
+            { unfold log_cons.
+              autorewrite with log_helpers.
+              rewrite putenv_proj_log; auto.
+              elim_eq_rect; simpl; auto.
+              rewrite may_read_proj_eq_may_read_lift in Heqb.
+              simpl_match; auto.
+            }
+            { elim_eq_rect; simpl.
+              rewrite may_read_proj_eq_may_read_lift in Heqb.
+              simpl_match; auto.
+            }
+          + _destruct.
+             { unfold log_cons.
+               autorewrite with log_helpers.
+               rewrite putenv_proj_log; auto.
+               rewrite log_app_comm_proj_log.
+               autorewrite with log_helpers.
+               elim_eq_rect; simpl; auto.
+               rewrite may_read_proj_eq_may_read_lift in Heqb.
+               simpl_match; auto.
+             }
+             { elim_eq_rect; simpl; auto.
+               rewrite may_read_proj_eq_may_read_lift in Heqb.
+               simpl_match; auto.
+             }
+        (* Write *)
+        - _start.
+          rewrite lift_action_preserves; auto.
+          unfold eq_rect_r.
+          _destruct.
+          { _destruct.
+            { unfold log_cons.
+              autorewrite with log_helpers.
+              rewrite putenv_proj_log; auto.
+              unfold eq_rect_r; destruct (pf_R_equal Rlift idx); simpl_eqs; simpl in *;
+                option_simpl; simplify_tuples; subst.
+              rewrite may_write_proj_eq_may_write_lift in Heqb.
+              rewrite Heqo. simpl_match. auto.
+            }
+            { destruct (pf_R_equal Rlift idx); simpl_eqs.
+              simpl_match.
+              rewrite may_write_proj_eq_may_write_lift in Heqb.
+              simpl_match; auto.
+            }
+          }
+          { destruct (pf_R_equal Rlift idx); simpl_eqs.
+            simpl_match; auto.
+          }
+        (* Unop *)
+        - _start.
+          rewrite lift_action_preserves; auto.
+          _destruct.
+        (* Binop *)
+        - _start.
+          rewrite lift_action_preserves; auto.
+          _destruct.
+          rewrite lift_action_preserves; auto.
+          _destruct.
+        (* ExternalCall *)
+        - _start.
+          rewrite lift_action_preserves; auto.
+          unfold eq_rect_r in *.
+          _destruct.
+          { rewrite H0. destruct (pf_R_equal Fnlift fn); simpl in *.
+            rewrite Heqo. auto.
+          }
+          { destruct (pf_R_equal Fnlift fn); simpl.
+            rewrite Heqo; auto.
+          }
+        (* InternalCall *)
+        - _start.
+          (* TODO: Can we do this with a lemma ... with ... ? *)
+          assert (
+           forall (sig argspec: tsig var_t) (args: acontext sig argspec)
+           (st': env_t REnv' R') gamma sched_log action_log,
+           (forall f, Sigma f = Sigma' (Fnlift.(rlift) f)) ->
+           (forall f, sigma f = rew [fun e : ExternalSignature => Sig_denote e] pf_R_equal Fnlift f in sigma' (Fnlift.(rlift) f)) ->
+           match interp_args (proj_env st') sigma gamma (proj_log sched_log) (proj_log action_log) args with
+           | Some (action_log0, results, Gamma) =>
+               exists log', interp_args st' sigma' gamma sched_log action_log
+                 (lift_args (@Lift.lift_action reg_t reg_t' R R' Rlift fn_name_t ext_fn_t ext_fn_t' Sigma Sigma' Fnlift)
+                    args) = Some (log', results, Gamma) /\
+                 action_log0 = proj_log log'
+           | None => interp_args st' sigma' gamma sched_log action_log
+                 (lift_args (sig := sig) (@Lift.lift_action reg_t reg_t' R R' Rlift fn_name_t ext_fn_t ext_fn_t' Sigma Sigma' Fnlift)
+                    args) = None
+           end) as lift_args_preserves.
+          { clear - lift_action_preserves.
+            induction args.
+            + simpl; intros; auto.
+              exists action_log; auto.
+            + intros; simpl. unfold opt_bind.
+              specialize IHargs with (st' := st') (gamma := gamma)
+                                                  (sched_log := sched_log) (action_log := action_log).
+              intuition.
+              _destruct; propositional.
+              { specialize lift_action_preserves with (action := v) (gamma := p1) (st' := st')
+                                                      (sched_log := sched_log) (action_log := log').
+                rewrite lift_action_preserves; auto.
+                unfold proj_interp_action_result.
+                simpl_match.
+                _destruct.
+                eexists; eauto.
+              }
+              { simpl_match. auto. }
+          }
+          { specialize lift_args_preserves with (st' := st') (gamma := gamma)
+                                              (sched_log := sched_log) (action_log := action_log) (args := args).
+            _destruct; propositional; simpl_match; auto.
+            rewrite lift_action_preserves; auto.
+            _destruct.
+          }
+        - _start.
+    Qed.
+
+  End LiftActionPreserves.
+
+  Lemma interp_rule_comm_proj :
+    forall rule (log_input: Log R' REnv'),
+    (forall f, Sigma f = Sigma' (Fnlift.(rlift) f)) ->
+    (forall f, sigma f = rew [fun e : ExternalSignature => Sig_denote e] pf_R_equal Fnlift f in sigma' (Fnlift.(rlift) f)) ->
+    match interp_rule (proj_env r') sigma (proj_log log_input) rule with
+    | Some l => exists l', interp_rule r' sigma' log_input (lift_rule rule) = Some l' /\
+                     proj_log l' = l
+    | None => interp_rule r' sigma' log_input (lift_rule rule) = None
+    end.
+  Proof.
+    unfold interp_rule.
+    intros.
+    rewrite<-@proj_log_empty with (Rlift := Rlift) (REnv' := REnv').
+    rewrite lift_action_preserves; auto.
+    unfold proj_interp_action_result.
+    fast_match_innermost_in_goal; auto.
+    - destruct_pairs. unfold lift_rule.
+      simpl_match. eexists; eauto.
+    - unfold lift_rule. simpl_match. reflexivity.
+  Qed.
+
+  Lemma interp_scheduler_delta'_comm_proj :
+    forall schedule (log_input acc_log: Log R' REnv'),
+    (forall rule, rules' (rule_name_lift rule) = lift_rule (rules rule)) ->
+    (forall f, Sigma f = Sigma' (Fnlift.(rlift) f)) ->
+    (forall f, sigma f = rew [fun e : ExternalSignature => Sig_denote e] pf_R_equal Fnlift f in sigma' (Fnlift.(rlift) f)) ->
+    interp_scheduler_delta' (REnv := REnv) (proj_env r') sigma rules
+                            (proj_log log_input) (proj_log acc_log) schedule =
+    proj_log (interp_scheduler_delta' r' sigma' rules' log_input acc_log (lift_scheduler rule_name_lift schedule)).
+  Proof.
+    induction schedule; simpl; intros; auto.
+    - intros. rewrite log_app_comm_proj_log.
+      pose proof interp_rule_comm_proj as Hrule.
+      match_innermost_in_goal;
+        specialize Hrule with (rule := rules r0) (log_input := log_app acc_log log_input);
+        rewrite Heqo in Hrule; intuition;
+        rewrite H; simpl_match.
+      + rewrite log_app_comm_proj_log; auto.
+      + auto.
+    - intros. rewrite log_app_comm_proj_log.
+      pose proof interp_rule_comm_proj as Hrule.
+      match_innermost_in_goal;
+        specialize Hrule with (rule := rules r0) (log_input := log_app acc_log log_input);
+        rewrite Heqo in Hrule; intuition;
+        rewrite H; simpl_match.
+      + rewrite log_app_comm_proj_log; auto.
+      + auto.
+  Qed.
+
+  Lemma interp_scheduler_delta_comm_proj :
+    forall schedule (log_input: Log R' REnv'),
+    (forall rule, rules' (rule_name_lift rule) = lift_rule (rules rule)) ->
+    (forall f, Sigma f = Sigma' (Fnlift.(rlift) f)) ->
+    (forall f, sigma f = rew [fun e : ExternalSignature => Sig_denote e] pf_R_equal Fnlift f in sigma' (Fnlift.(rlift) f)) ->
+    interp_scheduler_delta (REnv := REnv) (proj_env r') sigma rules (proj_log log_input) schedule =
+    proj_log
+      (interp_scheduler_delta r' sigma' rules' log_input (lift_scheduler rule_name_lift schedule)).
+  Proof.
+    unfold interp_scheduler_delta.
+    intros.
+    rewrite<-interp_scheduler_delta'_comm_proj; auto.
+    autorewrite with log_helpers; reflexivity.
+  Qed.
+
+  (* TODO: rename *)
+  Lemma log_app_interp_schedulre_delta_proj_comm_proj_interp_scheduler' :
+    forall schedule (log_input: Log R' REnv'),
+    (forall rule, rules' (rule_name_lift rule) = lift_rule (rules rule)) ->
+    (forall f, Sigma f = Sigma' (Fnlift.(rlift) f)) ->
+    (forall f, sigma f = rew [fun e : ExternalSignature => Sig_denote e] pf_R_equal Fnlift f in sigma' (Fnlift.(rlift) f)) ->
+    log_app (interp_scheduler_delta (proj_env r') sigma rules (proj_log log_input) schedule) (proj_log log_input) =
+    proj_log (interp_scheduler' r' sigma' rules' log_input (lift_scheduler rule_name_lift schedule)).
+  Proof.
+    intros.
+    rewrite interp_scheduler_delta_correspond_to_interp_scheduler.
+    rewrite interp_scheduler_delta_comm_proj; auto.
+    rewrite log_app_comm_proj_log. auto.
+  Qed.
+
+End Properties_LiftSchedule.
 
 Ltac lift_auto := auto with lift.
 
